secure_api/box/Box.PKAE.fst
@@ -1,23 +1,26 @@
+(**
+   Top level module of the verified implementation of NaCl's Crypto_box function.
+   This module contains the implementation of the actual crypto_box and crypto_box_open functions,
+   as well as some related types and helper functions.
+   Additionally, this module contains two tables that represent state in the modelling of PKAE.
+*)
 module Box.PKAE
 
-open Platform.Bytes
 open FStar.HyperHeap
 open FStar.HyperStack
 open Box.Flags
 open Box.AE
 open Box.DH
 open Box.PlainPKAE
-open Box.PlainAE
 open Box.Indexing
-open CoreCrypto
 
-module B = Platform.Bytes
 module MR = FStar.Monotonic.RRef
 module MM = MonotoneMap
 module HH = FStar.HyperHeap
 module HS = FStar.HyperStack
+module SPEC = Spec.SecretBox
 
-type rid = FStar.Monotonic.Seq.rid
+#set-options "--z3rlimit 100 --lax"
 
 assume val box_log_region: (r:MR.rid{ extends r root 
 					 /\ is_eternal_region r 
@@ -43,6 +46,17 @@ type box_log_key = (nonce*(i:id{AE_id? i /\ honest i}))
 type box_log_value = (protected_pkae_plain)
 type box_log_range = fun box_log_key -> box_log_value
 type box_log_inv (f:MM.map' box_log_key box_log_range) = True
+
+(**
+   This monotone map maps a tuple of (nonce*ciphertext) to a plaintext message. It is used if a message is
+   encrypted under an honest key while PKAE is idealized. During encryption, the plaintext will be stored in the log, indexed by the id and the nonce.
+   Upon decryption with an honest key, a lookup is performed in the log using the received pair of nonce and ciphertext as index. The log and its monotonic nature
+   guarantee the following properties, provided PKAE is idealized and the key is honest:
+   * Authenticity: Only the owner of the (honest) key can insert things into the log under a certain id. Anyone who decrypts a message with a key is thus
+     guaranteed that it was previously encrypted by another owner of that key.
+   * Uniqueness of nonces: Only one entry can exist for any combination of nonce and key. This means that a nonce can not be used a second time with the
+     same key.
+*)
 assume val box_log: MM.t box_log_region box_log_key box_log_range box_log_inv
 //let box_log = MM.alloc #pkae_table_region #pkae_table_key #pkae_table_range #pkae_table_inv
 
@@ -50,20 +64,35 @@ type box_key_log_key = i:id{AE_id? i /\ honest i}
 type box_key_log_value = (AE.key)
 type box_key_log_range = fun (i:box_key_log_key) -> (k:box_key_log_value{AE.get_index k = i})
 type box_key_log_inv (f:MM.map' box_key_log_key box_key_log_range) = True
+
+(**
+   This monotone map maps an AE id to a key. It is used when box_beforenm generates a key using an honest DH-public key and an honest DH-private key.
+   If PKAE is idealized, we box_beforenm generates a random key instead of computing it from its DH components. We thus need this monotone log to guarantee that 
+   for a given set of DH ids a single unique key is generated.
+*)
 assume val box_key_log:  MM.t box_key_log_region box_key_log_key box_key_log_range box_key_log_inv
 //let box_key_log = MM.alloc #pkae_table_region #pkae_table_key #pkae_table_range #pkae_table_inv
 
 
+(**
+   A PKAE public key, containing a DH public key.
+*)
 noeq abstract type pkae_pkey (pk_id:id{DH_id? pk_id}) =
   | PKey: dh_pk:dh_pkey{DH.pk_get_index dh_pk=pk_id} -> pkae_pkey pk_id
 
+(**
+   A PKAE private key, containing a DH private key.
+*)
 noeq abstract type pkae_skey (sk_id:id{DH_id? sk_id}) =
   | SKey: dh_sk:dh_skey{DH.sk_get_index dh_sk=sk_id} -> pkae_pk:pkae_pkey sk_id -> pkae_skey sk_id
 
+(**
+   Generate a PKAE keypair, consisting of a public and a private key.
+*)
 val keygen: #(i:id{DH_id? i}) -> ST (pkae_pkey i * pkae_skey i)
   (requires (fun h0 -> 
-  fresh i h0
-  /\ registered i
+    fresh i h0
+    /\ registered i
   ))
   (ensures (fun h0 res h1 -> 
     unfresh i
@@ -74,9 +103,17 @@ let keygen #i =
   let pkae_pk = PKey #i dh_pk in
   pkae_pk, SKey #i dh_sk pkae_pk
 
-
+(**
+   The type of the ciphertext that box and box_open use.
+*)
 type c = AE.cipher
 
+(**
+   Log invariant: WIP
+*)
+
+#reset-options
+#set-options "--z3rlimit 100"
 // TODO: We should be able to replace "dishonest i"  with "~(honest i)" everywhere!
 // TODO: Add patterns to quantifiers.
 let log_invariant_all_keys (h:mem) = 
@@ -99,11 +136,11 @@ let log_invariant_id (h:mem) (i:id) =
   /\ (forall (n:nonce) . (AE_id? i /\ honest i /\ (b2t pkae)) ==> (MM.fresh box_key_log i h ==> MM.fresh box_log (n,i) h)) // if it is not in the box_key_log, then there should be no nonces recorded in the box_log
 
 let log_invariant_single_key (h:mem) (i:id) (k:AE.key) =
-  ((AE_id? i /\ honest i /\ (b2t pkae)) ==> (forall (n:nonce) . (MM.defined box_key_log i h ==> (let k_log = get_logGT k in
+    ((AE_id? i /\ honest i /\ (b2t pkae)) ==> (forall (n:nonce) .{:pattern (MM.defined box_log (n,i) h) ; (MM.defined (get_logGT k) n h)} (MM.defined box_key_log i h ==> (let k_log = get_logGT k in
   								      (MM.defined box_log (n,i) h <==> MM.defined k_log n h)))))
   /\ (AE_id? i /\ honest i /\ (b2t pkae) /\ MM.defined box_key_log i h ==> (let k_log = get_logGT k in MR.m_contains k_log h))
 
-val recall_global_logs: unit -> ST unit
+private val recall_global_logs: unit -> ST unit
   (requires (fun h0 -> True))
   (ensures (fun h0 _ h1 -> 
     h0 == h1
@@ -119,7 +156,11 @@ let recall_global_logs () =
   MR.m_recall box_key_log
 
 
-#set-options "--z3rlimit 30"
+(**
+   box_beforenm is used to generate a key using a DH public and private key. The AE id of the resulting key is a combination of the DH ids of the
+   DH keys used to generate it. If idealized, the key resulting from this function will be random if both DH key ids are honest. To ensure that
+   only one key is generated per DH id pair, it is stored in the box_key_log and a lookup is performed before each key is generated.
+*)
 val box_beforenm: #(pk_id:id{DH_id? pk_id /\ registered pk_id}) -> 
 	              #(sk_id:id{DH_id? sk_id /\ registered sk_id}) -> 
 	              pk:pkae_pkey pk_id -> 
@@ -145,12 +186,11 @@ val box_beforenm: #(pk_id:id{DH_id? pk_id /\ registered pk_id}) ->
     /\ (honest i
       ==> (modifies regions_modified_honest_set h0 h1
     	 /\ MR.witnessed (MM.contains box_key_log i k))
-	 /\ MM.contains box_key_log i k h1)
+    	 /\ MM.contains box_key_log i k h1)
     /\ (dishonest i
       ==> (modifies regions_modified_dishonest_set h0 h1
-         /\ leak_key k = DH.prf_odhT sk.dh_sk pk.dh_pk))
+         /\ leak_key k = DH.prf_odhGT sk.dh_sk pk.dh_pk))
     /\ MR.m_contains k_log h1
-    /\ modifies regions_modified_honest_set h0 h1
     /\ log_invariant_single_key h1 i k
     /\ log_invariant_id h1 i
     /\ MR.m_contains id_log h1
@@ -165,131 +205,150 @@ let box_beforenm #pk_id #sk_id pk sk =
   if is_honest i then
     match MM.lookup box_key_log i with
     | Some k -> 
-	recall_global_logs();
+	//recall_global_logs();
+	MR.m_recall id_log;
+	MR.m_recall dh_key_log;
+	MR.m_recall box_log;
+	MR.m_recall box_key_log;
 	recall_log k;
         k
     | None ->
         let k = prf_odh sk.dh_sk pk.dh_pk in
         MM.extend box_key_log i k;
-	recall_global_logs();
+	//recall_global_logs();
+	MR.m_recall id_log;
+	MR.m_recall dh_key_log;
+	MR.m_recall box_log;
+	MR.m_recall box_key_log;
 	recall_log k;
         k
   else (
     let k = prf_odh sk.dh_sk pk.dh_pk in
-    recall_global_logs();
+    //recall_global_logs();
+    MR.m_recall id_log;
+    MR.m_recall dh_key_log;
+    MR.m_recall box_log;
+    MR.m_recall box_key_log;
     recall_log k;
     k)
 
 
-val box_afternm: k:AE.key ->
-		     n:nonce ->
-		     p:protected_pkae_plain{PlainPKAE.get_index p = AE.get_index k} ->
-		     ST c
-  (requires (fun h0 -> 
-    let k_log = get_logGT k in
-    let i = AE.get_index k in
-    MR.m_contains k_log h0
-    /\ MR.m_contains box_key_log h0
-    /\ MR.m_contains box_log h0
-    /\ log_invariant_single_key h0 i k
-    /\ log_invariant_id h0 i
-    /\ ((honest i /\ b2t pkae) ==> MM.fresh box_log (n,i) h0)
-    /\ ((honest i) ==> MM.defined box_key_log i h0)
-  ))
-  (ensures (fun h0 c h1 -> 
-    let i = AE.get_index k in
-    let k_log = get_logGT k in
-    let k_raw = get_keyGT k in
-    ((dishonest i \/ ~(b2t ae_ind_cca))
-      ==> c = CoreCrypto.aead_encryptT AES_128_CCM k_raw n empty_bytes (PlainPKAE.repr p))
-    /\ ((honest i /\ b2t ae_ind_cca)
-      ==> c = CoreCrypto.aead_encryptT AES_128_CCM k_raw n empty_bytes (createBytes (PlainPKAE.length p) 0z)
-	/\ MR.witnessed (MM.contains k_log n (c,ae_message_wrap p))
-	/\ MR.witnessed (MM.contains box_log (n,i) p))
-    /\ log_invariant_single_key h1 i k
-    /\ log_invariant_id h1 i
-  ))
-let box_afternm k n p =
-  MR.m_recall box_key_log;
-  MR.m_recall id_log;
-  MR.m_recall dh_key_log;
-  let i = AE.get_index k in
-  let ae_m = ae_message_wrap #i p in
-  let honest_i = is_honest i in
-  if honest_i && pkae then (
-    MM.extend box_log (n,i) p;
-    let c = AE.encrypt #i n k ae_m in
-    c
-  ) else (
-    let c = AE.encrypt #i n k ae_m in
-    c)
-  
-
-#set-options "--z3rlimit 25"
-val box: #(pk_id:id{DH_id? pk_id}) -> 
-	     #(sk_id:id{DH_id? sk_id}) -> 
-	     pk:pkae_pkey pk_id{registered pk_id} -> 
-	     sk:pkae_skey sk_id{registered sk_id} -> 
-	     n:nonce -> 
-	     p:protected_pkae_plain{PlainPKAE.get_index p = generate_ae_id pk_id sk_id} 
-	     -> ST c
-  (requires (fun h0 ->
-    let i = generate_ae_id pk_id sk_id in
-    registered i
-    // Liveness of global logs
-    /\ MR.m_contains box_log h0
-    /\ MR.m_contains id_log h0
-    /\ MR.m_contains box_key_log h0
-    /\ MR.m_contains dh_key_log h0
-    // Make sure that log_invariants hold.
-    /\ log_invariant_all_keys h0
-    /\ log_invariant_id h0 i
-    // Make sure that nonce is fresh
-    /\ ((honest i /\ b2t pkae) ==> MM.fresh box_log (n,i) h0)
-  ))
-  (ensures (fun h0 c h1 -> 
-    let i = generate_ae_id pk_id sk_id in
-    // Make sure that log_invariants hold. Would like to ensure "all_keys" variant, but too expensive to verify currently.
-    log_invariant_id h1 i
-    ///\ log_invariant_all_keys h1
-  ))
-let box #pk_id #sk_id pkae_pk pkae_sk n p =
-  let k = box_beforenm #pk_id #sk_id pkae_pk pkae_sk in
-  let c = box_afternm k n p in
-  c
-
-
-val box_open: #(sk_id:id{DH_id? sk_id}) -> 
-	     #(pk_id:id{DH_id? pk_id}) -> 
-	     n:nonce ->  
-	     sk:pkae_skey sk_id{registered sk_id} -> 
-	     pk:pkae_pkey pk_id{registered pk_id} -> 
-	     c:cipher{B.length c >= aeadTagSize AES_128_CCM} ->
-	     ST(option (p:protected_pkae_plain{PlainPKAE.get_index p = generate_ae_id pk_id sk_id}))
-  (requires (fun h0 ->
-    let i = generate_ae_id pk_id sk_id in
-    registered i
-    // Liveness of global logs
-    /\ MR.m_contains box_log h0
-    /\ MR.m_contains id_log h0
-    /\ MR.m_contains box_key_log h0
-    /\ MR.m_contains dh_key_log h0
-    // Make sure that log_invariants hold.
-    /\ log_invariant_all_keys h0
-    /\ log_invariant_id h0 i
-    // Make sure that nonce is fresh
-  ))
-  (ensures (fun h0 p h1 -> 
-    let i = generate_ae_id pk_id sk_id in
-    // Make sure that log_invariants hold. Would like to ensure "all_keys" variant, but too expensive to verify currently.
-    log_invariant_id h1 i
-    ///\ log_invariant_all_keys h1
-  ))
-let box_open #sk_id #pk_id n sk pk c =
-  let k = box_beforenm #pk_id #sk_id pk sk in
-  let i = AE.get_index k in
-  match AE.decrypt #i n k c with
-  | Some p -> 
-    let p' = (PlainAE.ae_message_unwrap #i p) in 
-    Some p'
-  | None -> None
+//(**
+//   box_afternm is used to encrypt a plaintext under an AE key using a nonce. If idealized and if the AE id is honest,
+//   the plaintext is stored in the box_log indexed by the AE id and the nonce.
+//*)
+//val box_afternm: k:AE.key ->
+//		     n:nonce ->
+//		     p:protected_pkae_plain{PlainPKAE.get_index p = AE.get_index k} ->
+//		     ST c
+//  (requires (fun h0 -> 
+//    let k_log = get_logGT k in
+//    let i = AE.get_index k in
+//    MR.m_contains k_log h0
+//    /\ MR.m_contains id_log h0
+//    /\ MR.m_contains box_log h0
+//    /\ MR.m_contains box_key_log h0
+//    /\ MR.m_contains dh_key_log h0
+//    /\ log_invariant_single_key h0 i k
+//    /\ log_invariant_id h0 i
+//    /\ ((honest i /\ b2t pkae) ==> MM.fresh box_log (n,i) h0)
+//    /\ ((honest i) ==> MM.defined box_key_log i h0)
+//  ))
+//  (ensures (fun h0 c h1 -> 
+//    let i = AE.get_index k in
+//    let k_log = get_logGT k in
+//    let k_raw = get_keyGT k in
+//    ((dishonest i \/ ~(b2t ae_ind_cca))
+//      ==> (c = SPEC.secretbox_easy (PlainPKAE.repr p) (AE.get_keyGT k) n))
+//    /\ ((honest i /\ b2t ae_ind_cca)
+//      ==> (c == SPEC.secretbox_easy (AE.create_zero_bytes (length p)) (AE.get_keyGT k) n
+//	/\ MR.witnessed (MM.contains k_log n (c,AE.message_wrap p))
+//	/\ MR.witnessed (MM.contains box_log (n,i) p)))
+//    /\ MR.m_contains id_log h1
+//    /\ MR.m_contains box_log h1
+//    /\ MR.m_contains box_key_log h1
+//    /\ MR.m_contains dh_key_log h1
+//    /\ log_invariant_single_key h1 i k
+//    /\ log_invariant_id h1 i
+//  ))
+//let box_afternm k n p =
+//  MR.m_recall box_key_log;
+//  MR.m_recall id_log;
+//  MR.m_recall dh_key_log;
+//  let i = AE.get_index k in
+//  let ae_m = AE.message_wrap #i p in
+//  let honest_i = is_honest i in
+//  if honest_i && pkae then (
+//    MM.extend box_log (n,i) p;
+//    let c = AE.encrypt #i n k ae_m in
+//    c
+//  ) else (
+//    let c = AE.encrypt #i n k ae_m in
+//    c)
+//
+//val box: #(pk_id:id{DH_id? pk_id}) -> 
+//	     #(sk_id:id{DH_id? sk_id}) -> 
+//	     pk:pkae_pkey pk_id{registered pk_id} -> 
+//	     sk:pkae_skey sk_id{registered sk_id} -> 
+//	     n:nonce -> 
+//	     p:protected_pkae_plain{PlainPKAE.get_index p = generate_ae_id pk_id sk_id} 
+//	     -> ST c
+//  (requires (fun h0 ->
+//    let i = generate_ae_id pk_id sk_id in
+//    registered i
+//    // Liveness of global logs
+//    /\ MR.m_contains box_log h0
+//    /\ MR.m_contains id_log h0
+//    /\ MR.m_contains box_key_log h0
+//    /\ MR.m_contains dh_key_log h0
+//    // Make sure that log_invariants hold.
+//    /\ log_invariant_all_keys h0
+//    /\ log_invariant_id h0 i
+//    // Make sure that nonce is fresh
+//    /\ ((honest i /\ b2t pkae) ==> MM.fresh box_log (n,i) h0)
+//  ))
+//  (ensures (fun h0 c h1 -> 
+//    let i = generate_ae_id pk_id sk_id in
+//    // Make sure that log_invariants hold. Would like to ensure "all_keys" variant, but too expensive to verify currently.
+//    log_invariant_id h1 i
+//    ///\ log_invariant_all_keys h1
+//  ))
+//let box #pk_id #sk_id pkae_pk pkae_sk n p =
+//  let k = box_beforenm #pk_id #sk_id pkae_pk pkae_sk in
+//  let c = box_afternm k n p in
+//  c
+//
+//
+//val box_open: #(sk_id:id{DH_id? sk_id}) -> 
+//	     #(pk_id:id{DH_id? pk_id}) -> 
+//	     n:nonce ->  
+//	     sk:pkae_skey sk_id{registered sk_id} -> 
+//	     pk:pkae_pkey pk_id{registered pk_id} -> 
+//	     c:cipher ->
+//	     ST(option (p:protected_pkae_plain))
+//  (requires (fun h0 ->
+//    let i = generate_ae_id pk_id sk_id in
+//    registered i
+//    // Liveness of global logs
+//    /\ MR.m_contains box_log h0
+//    /\ MR.m_contains id_log h0
+//    /\ MR.m_contains box_key_log h0
+//    /\ MR.m_contains dh_key_log h0
+//    // Make sure that log_invariants hold.
+//    /\ log_invariant_all_keys h0
+//    /\ log_invariant_id h0 i
+//  ))
+//  (ensures (fun h0 p h1 -> 
+//    let i = generate_ae_id pk_id sk_id in
+//    // Make sure that log_invariants hold. Would like to ensure "all_keys" variant, but too expensive to verify currently.
+//    log_invariant_id h1 i
+//    ///\ log_invariant_all_keys h1
+//  ))
+//let box_open #sk_id #pk_id n sk pk c =
+//  let k = box_beforenm #pk_id #sk_id pk sk in
+//  let i = AE.get_index k in
+//  match AE.decrypt #i n k c with
+//  | Some p -> 
+//    let p' = (AE.message_unwrap #i p) in 
+//    Some p'
+//  | None -> None
